more

haskell/Traverse.hs
@@ -1,0 +1,30 @@
+{-# LANGUAGE DeriveFunctor      #-}
+
+data List a = Nil | Cons a (List a)
+    deriving (Functor)
+
+-- some implementation of traverse
+traverse1 :: (Applicative f) => (a -> f b) -> List a -> f (List b)
+traverse1 _ Nil = pure Nil
+traverse1 f (Cons x xs) = Cons <$> (f x) <*> (traverse1 f xs)  
+
+-- some implementation of sequenceA
+sequenceA1 :: (Applicative f) => List (f a) -> f (List a)
+sequenceA1 Nil = pure Nil
+sequenceA1 (Cons x xs) = Cons <$> x <*> sequenceA1 xs
+
+-- traverse can be implemented in terms of sequenceA
+traverse2 :: (Applicative f) => (a -> f b) -> List a -> f (List b)
+traverse2 = (.) sequenceA1 . fmap
+
+-- sequenceA can be implemented in terms of traverse
+sequenceA2 :: (Applicative f) => List (f a) -> f (List a)
+sequenceA2 = traverse1 id
+
+-- MapM is just the same as traverse for monadic actions
+mapM1 :: (Monad m) => (a -> m b) -> List a -> m (List b)
+mapM1 = traverse1
+
+-- sequence is just sequenceA for lists of mandic actions
+sequence1 :: (Monad m) => List (m a) -> m (List a)
+sequence1 = sequenceA1 
