coq/Logic/Rel/Properties.v
@@ -1,35 +1,69 @@
+Require Import Logic.Axiom.Extensionality.
+
 Require Import Logic.Rel.R. 
+Require Import Logic.Rel.Converse.
+Require Import Logic.Rel.Composition.
 
 (* Reflexive predicate on Rel a                                                 *)
 Definition reflexive (a:Type) (r:Rel a) : Prop := forall (x:a), 
     r x x.
 
-Arguments reflexive {a} _.
+Arguments reflexive {a}.
 
 (* Symmetric predicate on Rel a                                                 *)
 Definition symmetric (a:Type) (r:Rel a) : Prop := forall (x y:a), 
     r x y -> r y x.
 
-Arguments symmetric {a} _.
+Arguments symmetric {a}.
 
 (* Transitive predicate on Rel a                                                *)
 Definition transitive (a:Type) (r:Rel a) : Prop := forall (x y z:a), 
     r x y -> r y z -> r x z.
 
-Arguments transitive {a} _.
+Arguments transitive {a}.
 
 Definition antisymmetric (a:Type) (r:Rel a) : Prop := forall (x y:a),
     r x y -> r y x -> x = y.
 
-Arguments antisymmetric {a} _.
+Arguments antisymmetric {a}.
 
 (* Equivalence predicate on Rel a                                               *)
 Definition equivalence (a:Type) (r:Rel a) : Prop := 
     reflexive r /\ symmetric r /\ transitive r.
 
-Arguments equivalence {a} _.
+Arguments equivalence {a}.
 
 Definition partial_order (a:Type) (r:Rel a) : Prop :=
     reflexive r /\ antisymmetric r /\ transitive r.
 
-Arguments partial_order {a} _.
+Arguments partial_order {a}.
+
+Definition idempotent (a:Type) (r:Rel a) : Prop := 
+    r ; r = r.
+
+Arguments idempotent {a}.
+
+Lemma sym_trans_idem : forall (a:Type) (r:Rel a), 
+    symmetric r -> transitive r -> idempotent r.
+Proof.
+    intros a r H1 H2. apply Ext. intros x y. split; intros H3.
+    - destruct H3 as [z [H3 H4]]. apply H2 with z; assumption.
+    - exists x. split; try assumption.
+      apply H2 with y; try assumption. apply H1. assumption.
+Qed.
+
+Lemma sym_trans_conv : forall (a:Type) (r:Rel a),
+    (symmetric r /\ transitive r) <-> r = r ; conv r.
+Proof.
+    intros a r. split; intros H1.
+    - destruct H1 as [H1 H2]. apply Ext. intros x y. split; intros H3.
+        + exists x. split; try assumption. apply H2 with y; try assumption.
+          apply H1. assumption.
+        + destruct H3 as [z [H3 H4]]. apply H2 with z; try assumption.
+          apply H1. assumption.
+    - assert (symmetric r) as H2.
+        { intros x y H3. rewrite H1 in H3. destruct H3 as [z [H3 H4]].
+          rewrite H1. exists z. split; assumption. }
+      split; try assumption. intros x y z H3 H4. rewrite H1. exists y.
+      split; try assumption. apply H2. assumption.
+Qed.
